---
permalink: /.ttl
---
@prefix cs: <https://linked.data.gov.au/def/reg-roles> .
@prefix rdf:  <http://www.w3.org/1999/02/22-rdf-syntax-ns#> .
@prefix rdfs: <http://www.w3.org/2000/01/rdf-schema#> .
@prefix owl:  <http://www.w3.org/2002/07/owl#> .
@prefix xsd:  <http://www.w3.org/2001/XMLSchema#> .
@prefix sdo: <https://schema.org/> .
@prefix skos: <http://www.w3.org/2004/02/skos/core#> .
@prefix reg:  <http://purl.org/linked-data/registry#> .
@prefix dcterms:  <http://purl.org/dc/terms/> .
@prefix vann: <http://purl.org/vocab/vann/> .
@prefix : <https://linked.data.gov.au/def/reg-roles/> .


<https://linked.data.gov.au/def/reg-roles> 
    a owl:Ontology , skos:ConceptScheme;
    skos:prefLabel "Registry Roles Vocabulary"@en ;
    skos:definition """This vocabulary is a flat - no hiearchy - listing of the roles for people and organisations defined within the ISO standard 19135 "Geographic information â€” Procedures for item registration ISO/DIS 19135-1" https://www.iso.org/standard/54721.html."""@en ;
    owl:versionIRI <https://linked.data.gov.au/def/reg-roles/1.0> ;
    owl:versionInfo "1.0"@en ;
    dcterms:contributor <https://orcid.org/0000-0002-8742-7730>;
    vann:preferredNamespaceUri "https://linked.data.gov.au/def/reg-roles/"^^xsd:string ;
    dcterms:creator <http://orcid.org/0000-0002-8742-7730> ;
    vann:preferredNamespacePrefix "reg-roles"@en ;
    dcterms:publisher <https://linked.data.gov.au/org/agldwg> ;
    rdfs:seeAlso <https://github.com/AGLDWG/reg-roles> ;
    dcterms:issued "2021-11-03"^^xsd:date ;
    dcterms:modified "2021-11-05"^^xsd:date ;
    dcterms:rights "(c) Commonwealth of Australia 2021"@en ;
    dcterms:created "2021-11-03"^^xsd:date ;
    dcterms:source "https://www.iso.org/standard/54721.html"^^xsd:anyURI ;
    skos:hasTopConcept 
        :control-body ,
        :register-manager ,
        :register-owner ,
        :register-user ,
        :registry-manager ,
        :submitter ,
        :submitting-organization ;
.

<https://linked.data.gov.au/def/agldwg>
    a sdo:Organization ;
    sdo:name "Australian Government Linked Data Working Group" ;
    sdo:url "http://www.linked.data.gov.au"^^xsd:anyURI ;
.

<https://orcid.org/0000-0002-8742-7730>
    a sdo:Person ;
    sdo:honorificPrefix "Dr" ;
    sdo:name "Nicholas J. Car" ;
    sdo:email "nicholas.car@surroundaustralia.com"^^xsd:anyURI ;
    sdo:affiliation <https://linked.data.gov.au/org/surround> ;
.


:control-body
    a skos:Concept ;
    skos:prefLabel "Control Body"@en;
    skos:definition "Group of technical experts that makes decisions regarding the content of a Register."@en;
    skos:inScheme cs: ;
    rdfs:isDefinedBy cs: ;
    skos:topConceptOf cs: ;
.

:register-manager
    a skos:Concept ;
    skos:prefLabel "Register Manager"@en;
    skos:definition "Organization to which management of a Register has been delegated by the **Register Owner**."@en;
    skos:inScheme cs: ;
    rdfs:isDefinedBy cs: ;
    skos:topConceptOf cs: ;
.

:register-owner
    a skos:Concept ;
    skos:prefLabel "Register Owner"@en;
    skos:definition "Organization that establishes a Register."@en;
    skos:inScheme cs: ;
    rdfs:isDefinedBy cs: ;
    skos:topConceptOf cs: ;
.

:register-user
    a skos:Concept ;
    skos:prefLabel "Register User"@en;
    skos:definition "Users of a Register without another defined role."@en;
    skos:inScheme cs: ;
    rdfs:isDefinedBy cs: ;
    skos:topConceptOf cs: ;
.

:registry-manager
    a skos:Concept ;
    skos:prefLabel "Registry Manager"@en;
    skos:definition "A registry manager is a person or an organization responsible for the day-to-day management of a registry"@en;
    skos:inScheme cs: ;
    rdfs:isDefinedBy cs: ;
    skos:topConceptOf cs: ;
.

:submitter
    a skos:Concept ;
    skos:prefLabel "Submitter"@en;
    skos:definition "Person requesting changes to a Register on behalf of a **Submitting Organization**."@en;
    skos:inScheme cs: ;
    rdfs:isDefinedBy cs: ;
    skos:topConceptOf cs: ;
.

:submitting-organization
    a skos:Concept ;
    skos:prefLabel "Submitting Organization"@en;
    skos:definition "Organization authorized by a **Register Owner** to propose changes to the content of a Register."@en;
    skos:inScheme cs: ;
    rdfs:isDefinedBy cs: ;
    skos:topConceptOf cs: ;
.
